backend/Asmgenproof0.v
@@ -862,7 +862,7 @@ Lemma exec_straight_steps_1:
   Genv.find_funct_ptr ge b = Some (Internal fn) ->
   Genv.find_comp ge (Vptr b Ptrofs.zero) = (comp_of fn) ->
   code_tail (Ptrofs.unsigned ofs) (fn_code fn) c ->
-  plus step ge (State s rs m) E0 (State s rs' m').
+  plus step ge (State s rs m true) E0 (State s rs' m' true).
 Proof.
   induction 1; intros.
   apply plus_one.
